runningexample verifies.. but won't run yet

io/Compiler.Examples.fst
@@ -9,14 +9,14 @@ open FStar.List
 open Compiler.Model
 
 (** Utils **)
-type source_arrow (arg:Type u#a) (res:Type u#b) (pre:arg -> trace -> Type0) (post:arg -> trace -> resexn res -> trace -> Type0) (fl:erased tflag) =
-  x:arg -> MIO (resexn res) fl (pre x) (post x)
+type source_arrow (mst:mst) (arg:Type u#a) (res:Type u#b) (pre:arg -> trace -> Type0) (post:arg -> trace -> resexn res -> trace -> Type0) (fl:erased tflag) =
+  x:arg -> MIO (resexn res) mst fl (pre x) (post x)
 
 type c1typ (#arg:Type u#a) (#res:Type u#b) (pre:arg -> trace -> Type0) (post:arg -> trace -> resexn res -> trace -> Type0) (pi:policy_spec) =
   squash (forall x h lt. pre x h /\ enforced_locally pi h lt ==> post x h (Inr Contract_failure) lt)
   
-type c2typ (#arg:Type u#a) (#res:Type u#b) (pre:arg -> trace -> Type0) (post:arg -> trace -> resexn res -> trace -> Type0) (pi:policy_spec) (rc:rc_typ arg (resexn res)) =
-  squash (forall x h lt r. pre x h /\ enforced_locally pi h lt /\ rc x h r lt ==> post x h r lt)
+type c2typ (#arg:Type u#a) (#res:Type u#b) (pre:arg -> trace -> Type0) (post:arg -> trace -> resexn res -> trace -> Type0) (pi:policy_spec) (irc:irc_typ arg (resexn res)) =
+  squash (forall x h lt r. pre x h /\ enforced_locally pi h lt /\ irc x h r lt ==> post x h r lt)
 
 type stronger_pis (pi1:policy_spec) (pi2:policy_spec) =
   squash (forall h lt. enforced_locally pi1 h lt ==> enforced_locally pi2 h lt)
@@ -28,7 +28,12 @@ let test1_pre = (fun () h -> True)
 let test1_post = (fun () h (rfd:resexn file_descr) lt -> 
   (forall fd'. ~((EOpenfile false "/etc/passwd" fd') `List.memP` lt)) /\ (Inl? rfd ==> is_open (Inl?.v rfd) (rev lt @ h)))
 
-type test1_ct = source_arrow unit file_descr test1_pre test1_post
+let mst1 : mst = {
+  cst = list file_descr;
+  models = (fun s h -> forall fd. memP fd s <==> is_open fd h);
+}
+
+type test1_ct = source_arrow mst1 unit file_descr test1_pre test1_post
 
 let test1_pi : policy_spec = 
   fun h isTrusted cmd arg -> 
@@ -37,17 +42,25 @@ let test1_pi : policy_spec =
     | Openfile -> (arg <> "/etc/passwd")
     | _ -> True)
 
-let test1_phi : policy test1_pi =
+let test1_phi : policy mst1 test1_pi =
   fun h cmd arg -> 
     match cmd, arg with 
-    | Openfile, s -> 
+    | Openfile, s ->
       if s = "/etc/passwd" then false 
       else true 
     | _ -> true
-    
-let test1_ct_rc = (fun () h (rfd:resexn file_descr) lt -> Inl? rfd && (is_open (Inl?.v rfd) (rev lt @ h)))
-let test1_ct_rcs : tree pck_rc = 
-  Node (| unit, resexn file_descr, test1_ct_rc |) 
+
+let test1_ct_irc : irc_typ unit (resexn file_descr) =
+  fun () h (rfd:resexn file_descr) lt -> Inl? rfd && (is_open (Inl?.v rfd) (rev lt @ h))
+
+let test1_ct_rc : rc_typ mst1 test1_ct_irc =
+  fun () s0 rfd s1 ->
+    match rfd with
+    | Inl fd -> List.mem fd s1
+    | Inr _ -> false
+
+let test1_ct_rcs : tree (pck_rc mst1) = 
+  Node (| unit, resexn file_descr, test1_ct_irc, test1_ct_rc |) 
     Leaf 
     Leaf
 
@@ -62,12 +75,14 @@ let test1_c1post =
     | e :: tail -> aux (e::h) tail) in
   Classical.forall_intro_2 (Classical.move_requires_2 aux)
 
-assume val test1_c2post : c2typ test1_pre test1_post test1_pi test1_ct_rc
+assume val test1_c2post : c2typ test1_pre test1_post test1_pi test1_ct_irc
 //let test1_c2post = ()
 
-let test1_ct_importable (fl:erased tflag) : safe_importable (test1_ct fl) test1_pi test1_ct_rcs fl =
+#set-options "--print_implicits"
+
+let test1_ct_importable (fl:erased tflag) : safe_importable (test1_ct fl) mst1 test1_pi test1_ct_rcs fl =
   safe_importable_arrow_pre_post_args_res _ _ test1_c1post test1_c2post #exportable_unit #importable_file_descr
-                                                  
+
 val test1_stronger_pis : stronger_pis test1_pi test1_pi
 let test1_stronger_pis = 
   let rec aux (h:trace) (lt:trace) : Lemma
@@ -79,7 +94,7 @@ let test1_stronger_pis =
   Classical.forall_intro_2 (Classical.move_requires_2 aux)
 
 [@@ (postprocess_with (fun () -> norm [delta_only [`%test1_ct; `%source_arrow; `%test1_ct_importable]]; trefl ()))]
-let test1 : src_interface = {
+let test1 : src_interface mst1 = {
   pi = test1_pi; phi = test1_phi;
 
   ct = test1_ct;
@@ -89,142 +104,148 @@ let test1 : src_interface = {
   psi = (fun _ _ lt -> (forall fd'. ~((EOpenfile false "/etc/passwd" fd') `List.memP` lt)));
 }
 
-val test1_prog : prog_src test1
-let test1_prog #fl ctx () : MIO int (fl + IOActions) (fun _ -> True) test1.psi =
+val test1_prog : prog_src mst1 test1
+let test1_prog #fl ctx () : MIO int mst1 (fl + IOActions) (fun _ -> True) test1.psi =
   //let test = static_cmd Openfile "/etc/passwd" in
   let _ = ctx () in
   0 
 
-val test1_ctx : ctx_src test1
-let test1_ctx #fl io_acts eff_rcs () : MIO (resexn file_descr) fl (fun _ -> True) (test1_post ()) = 
+val test1_ctx : ctx_src mst1 test1
+#push-options "--compat_pre_core 1"
+let test1_ctx #fl io_acts eff_rcs () : MIO (resexn file_descr) mst1 fl (fun _ -> True) (test1_post ()) = 
   io_acts Openfile "/etc/passwd"
+#pop-options
 
-val test1_ctx_t : ctx_tgt (comp_int_src_tgt test1)
-let test1_ctx_t #fl io_acts () : MIOpi (resexn file_descr) fl test1_pi =
+val test1_ctx_t : ctx_tgt mst1 (comp_int_src_tgt mst1 test1)
+#push-options "--compat_pre_core 1"
+let test1_ctx_t #fl io_acts () : MIOpi (resexn file_descr) mst1 fl test1_pi =
   io_acts Openfile "/etc/passwd"
+#pop-options
 
-(** ** Test 2 - HO left 1 **)
-let test2_pi : policy_spec = (fun _ _ _ _ -> true)
-let test2_phi : policy test2_pi = (fun _ _ _ -> true)
-
-let test2_cb (fl:erased tflag) = (fd:file_descr -> MIO (resexn unit) fl (fun h -> is_open fd h) (fun _ _ lt -> lt == []))
-let test2_post = (fun _ h (rfd:resexn file_descr) lt -> Inl? rfd ==> is_open (Inl?.v rfd) (rev lt @ h))
-let test2_ct (fl:erased tflag) = (cb:test2_cb fl) -> MIO (resexn file_descr) fl (fun _ -> True) (test2_post cb)
-
-let test2_rcs : tree pck_rc =  
-  Node (| unit, resexn file_descr, (fun () h (rfd:resexn file_descr) lt -> Inl? rfd && (is_open (Inl?.v rfd) (rev lt @ h))) |) 
-     (Node (| file_descr, unit, (fun fd h _ _ -> is_open fd h) |) Leaf Leaf)
-     Leaf
-  
-assume val test2_c1post : #a:Type -> squash (forall (x:a) h lt. enforced_locally test2_pi h lt ==> (exists r. test2_post x h r lt))
-
-val test2_c2post : #a:Type -> squash (forall (x:a) h r lt. enforced_locally test2_pi h lt /\ ((Mkdtuple3?._3 (root test2_rcs)) () h r lt) ==> test2_post x h r lt)
-let test2_c2post #a = ()
-
-let test2_ct_importable (fl:erased tflag) : safe_importable (test2_ct fl) test2_pi test2_rcs fl = 
-  let exportable_cb = exportable_arrow_pre_post_args file_descr unit #test2_pi #(left test2_rcs) #fl (fun fd h -> is_open fd h) (fun fd _ _ lt -> lt == []) in
-  safe_importable_arrow_pre_post_res
-    (fun _ _ -> True)  (** pre **)
-    test2_post       (** post **)
-    (test2_c1post #(test2_cb fl))
-    (test2_c2post #(test2_cb fl))
-    #exportable_cb
-    #importable_file_descr
-
-[@@ (postprocess_with (fun () -> norm [delta_only [`%test2_ct; `%test2_cb;`%test2_ct_importable]]; trefl ()))]
-let test2 : src_interface = {
-  pi = test2_pi; phi = test2_phi; 
-  ct = test2_ct; ct_rcs = test2_rcs; ct_importable = test2_ct_importable; 
-  psi = (fun _ _ _ -> True);
-}
-
-val test2_prog : prog_src test2
-let test2_prog #fl ctx () =
-  let _ = ctx (fun fd -> Inl ()) in
-  (** return exit code **) 0
-
-val test2_ctx : ctx_src test2 
-let test2_ctx #fl io_acts eff_rcs cb : MIO (resexn file_descr) fl (fun _ -> True) (fun h rfd lt -> Inl? rfd ==> is_open (Inl?.v rfd) (rev lt @ h)) = 
-  let post1 = root eff_rcs in
-  let (| _, pre1 |) = root (left eff_rcs) in 
-  let rfd = io_acts Openfile "/etc/passwd" in
-  match rfd with
-  | Inl fd -> let _ = pre1 fd in rfd
-  | _ -> rfd
-
-val test2_ctx_t : ctx_tgt (comp_int_src_tgt test2)
-let test2_ctx_t #fl io_acts cb : MIOpi (resexn file_descr) fl (comp_int_src_tgt test2).pi = 
-  let rfd = io_acts Openfile "/etc/passwd" in
-  match rfd with
-  | Inl fd -> begin
-    //let _ = io_acts Close fd in 
-    let _ = cb fd in 
-    rfd
-  end
-  | _ -> rfd
-
-(** ** Test 3 - HO right 1 **)
-let test3_pi : policy_spec = (fun _ _ _ _ -> true)
-let test3_phi : policy test3_pi = (fun _ _ _ -> true)
-
-let test3_cb (fl:erased tflag) = (fd:file_descr -> MIO (resexn unit) fl (fun h -> True) (fun _ _ lt -> True))
-let test3_post #a = (fun (x:file_descr) h (r:a) lt -> True)
-let test3_ct (fl:erased tflag) = x:file_descr -> MIO (resexn (test3_cb fl)) fl (fun _ -> True) (test3_post x)
-
-let test3_rcs : tree pck_rc =  
-  Node (| file_descr, unit, (fun x h r lt -> true) |) 
-     Leaf
-     (Node (| file_descr, resexn unit, (fun fd h _ _ -> true) |) Leaf Leaf)
-
-let test3_cb_importable (fl:erased tflag) : safe_importable (test3_cb fl) test3_pi (right test3_rcs) fl = 
-  safe_importable_arrow_pre_post_args_res
-    #file_descr #unit
-    #test3_pi
-    #(right test3_rcs)
-    #fl
-    (fun fd h -> True)
-    (fun fd _ _ lt -> True)
-    ()
-    ()
-    #exportable_file_descr
-    #importable_unit
-  
-assume val test3_c1post : #a:Type -> squash (forall x h lt. enforced_locally test3_pi h lt ==> (exists (r:a). test3_post x h r lt))
-//let test3_c1post #a = () 
-val test3_c2post : #a:Type -> squash (forall x h (r:a) lt. enforced_locally test3_pi h lt /\ ((Mkdtuple3?._3 (root test3_rcs)) x h () lt) ==> test3_post x h r lt)
-let test3_c2post #a = ()
-
-let test3_ct_importable (fl:erased tflag) : safe_importable (test3_ct fl) test3_pi test3_rcs fl = 
-  safe_importable_arrow_pre_post_args
-    #file_descr #(test3_cb fl) #test3_pi #test3_rcs #fl
-    (fun _ _ -> True)  (** pre **)
-    test3_post       (** post **)
-    (test3_c1post #(test3_cb fl))
-    (test3_c2post #(test3_cb fl))
-    #exportable_file_descr
-    #(safe_importable_is_importable (test3_cb_importable fl))
-
-[@@ (postprocess_with (fun () -> norm [delta_only [`%test3_ct; `%test3_cb;`%test3_ct_importable]]; trefl ()))]
-let test3 : src_interface = {
-  pi = test3_pi; phi = test3_phi;
-  ct = test3_ct; ct_rcs = test3_rcs; ct_importable = test3_ct_importable; 
-  psi = (fun _ _ _ -> True);
-}
-
-val test3_prog : prog_src test3
-let test3_prog #fl ctx () : MIO int (IOActions + fl) (fun _ -> True) (fun _ _ _ -> True) =
-  match static_cmd true Openfile "test.txt" with
-  | Inl fd -> begin
-    match ctx fd with
-    | Inl cb -> let _ : resexn unit = cb fd in 0
-    | Inr err -> -1
-    end
-  | Inr err -> -1
-
-val test3_ctx : ctx_src test3 
-let test3_ctx #fl io_acts eff_rcs fd = 
-  Inl (fun (fd:file_descr) -> Inl () <: (MIOwp (resexn unit) fl trivial_hist))
-
-val test3_ctx_t : ctx_tgt (comp_int_src_tgt test3)
-let test3_ctx_t #fl io_acts fd : MIOpi (resexn (file_descr -> MIOpi (resexn unit) fl test3_pi)) fl test3_pi = 
-  Inl (fun (fd:file_descr) -> Inl () <: (MIOpi (resexn unit) fl test3_pi))
+// 
+// 
+// (** ** Test 2 - HO left 1 **)
+// let test2_pi : policy_spec = (fun _ _ _ _ -> true)
+// let test2_phi : policy test2_pi = (fun _ _ _ -> true)
+// 
+// let test2_cb (fl:erased tflag) = (fd:file_descr -> MIO (resexn unit) fl (fun h -> is_open fd h) (fun _ _ lt -> lt == []))
+// let test2_post = (fun _ h (rfd:resexn file_descr) lt -> Inl? rfd ==> is_open (Inl?.v rfd) (rev lt @ h))
+// let test2_ct (fl:erased tflag) = (cb:test2_cb fl) -> MIO (resexn file_descr) fl (fun _ -> True) (test2_post cb)
+// 
+// let test2_rcs : tree pck_rc =  
+//   Node (| unit, resexn file_descr, (fun () h (rfd:resexn file_descr) lt -> Inl? rfd && (is_open (Inl?.v rfd) (rev lt @ h))) |) 
+//      (Node (| file_descr, unit, (fun fd h _ _ -> is_open fd h) |) Leaf Leaf)
+//      Leaf
+//   
+// assume val test2_c1post : #a:Type -> squash (forall (x:a) h lt. enforced_locally test2_pi h lt ==> (exists r. test2_post x h r lt))
+// 
+// val test2_c2post : #a:Type -> squash (forall (x:a) h r lt. enforced_locally test2_pi h lt /\ ((Mkdtuple3?._3 (root test2_rcs)) () h r lt) ==> test2_post x h r lt)
+// let test2_c2post #a = ()
+// 
+// let test2_ct_importable (fl:erased tflag) : safe_importable (test2_ct fl) test2_pi test2_rcs fl = 
+//   let exportable_cb = exportable_arrow_pre_post_args file_descr unit #test2_pi #(left test2_rcs) #fl (fun fd h -> is_open fd h) (fun fd _ _ lt -> lt == []) in
+//   safe_importable_arrow_pre_post_res
+//     (fun _ _ -> True)  (** pre **)
+//     test2_post       (** post **)
+//     (test2_c1post #(test2_cb fl))
+//     (test2_c2post #(test2_cb fl))
+//     #exportable_cb
+//     #importable_file_descr
+// 
+// [@@ (postprocess_with (fun () -> norm [delta_only [`%test2_ct; `%test2_cb;`%test2_ct_importable]]; trefl ()))]
+// let test2 : src_interface = {
+//   pi = test2_pi; phi = test2_phi; 
+//   ct = test2_ct; ct_rcs = test2_rcs; ct_importable = test2_ct_importable; 
+//   psi = (fun _ _ _ -> True);
+// }
+// 
+// val test2_prog : prog_src test2
+// let test2_prog #fl ctx () =
+//   let _ = ctx (fun fd -> Inl ()) in
+//   (** return exit code **) 0
+// 
+// val test2_ctx : ctx_src test2 
+// let test2_ctx #fl io_acts eff_rcs cb : MIO (resexn file_descr) fl (fun _ -> True) (fun h rfd lt -> Inl? rfd ==> is_open (Inl?.v rfd) (rev lt @ h)) = 
+//   let post1 = root eff_rcs in
+//   let (| _, pre1 |) = root (left eff_rcs) in 
+//   let rfd = io_acts Openfile "/etc/passwd" in
+//   match rfd with
+//   | Inl fd -> let _ = pre1 fd in rfd
+//   | _ -> rfd
+// 
+// val test2_ctx_t : ctx_tgt (comp_int_src_tgt test2)
+// let test2_ctx_t #fl io_acts cb : MIOpi (resexn file_descr) fl (comp_int_src_tgt test2).pi = 
+//   let rfd = io_acts Openfile "/etc/passwd" in
+//   match rfd with
+//   | Inl fd -> begin
+//     //let _ = io_acts Close fd in 
+//     let _ = cb fd in 
+//     rfd
+//   end
+//   | _ -> rfd
+// 
+// (** ** Test 3 - HO right 1 **)
+// let test3_pi : policy_spec = (fun _ _ _ _ -> true)
+// let test3_phi : policy test3_pi = (fun _ _ _ -> true)
+// 
+// let test3_cb (fl:erased tflag) = (fd:file_descr -> MIO (resexn unit) fl (fun h -> True) (fun _ _ lt -> True))
+// let test3_post #a = (fun (x:file_descr) h (r:a) lt -> True)
+// let test3_ct (fl:erased tflag) = x:file_descr -> MIO (resexn (test3_cb fl)) fl (fun _ -> True) (test3_post x)
+// 
+// let test3_rcs : tree pck_rc =  
+//   Node (| file_descr, unit, (fun x h r lt -> true) |) 
+//      Leaf
+//      (Node (| file_descr, resexn unit, (fun fd h _ _ -> true) |) Leaf Leaf)
+// 
+// let test3_cb_importable (fl:erased tflag) : safe_importable (test3_cb fl) test3_pi (right test3_rcs) fl = 
+//   safe_importable_arrow_pre_post_args_res
+//     #file_descr #unit
+//     #test3_pi
+//     #(right test3_rcs)
+//     #fl
+//     (fun fd h -> True)
+//     (fun fd _ _ lt -> True)
+//     ()
+//     ()
+//     #exportable_file_descr
+//     #importable_unit
+//   
+// assume val test3_c1post : #a:Type -> squash (forall x h lt. enforced_locally test3_pi h lt ==> (exists (r:a). test3_post x h r lt))
+// //let test3_c1post #a = () 
+// val test3_c2post : #a:Type -> squash (forall x h (r:a) lt. enforced_locally test3_pi h lt /\ ((Mkdtuple3?._3 (root test3_rcs)) x h () lt) ==> test3_post x h r lt)
+// let test3_c2post #a = ()
+// 
+// let test3_ct_importable (fl:erased tflag) : safe_importable (test3_ct fl) test3_pi test3_rcs fl = 
+//   safe_importable_arrow_pre_post_args
+//     #file_descr #(test3_cb fl) #test3_pi #test3_rcs #fl
+//     (fun _ _ -> True)  (** pre **)
+//     test3_post       (** post **)
+//     (test3_c1post #(test3_cb fl))
+//     (test3_c2post #(test3_cb fl))
+//     #exportable_file_descr
+//     #(safe_importable_is_importable (test3_cb_importable fl))
+// 
+// [@@ (postprocess_with (fun () -> norm [delta_only [`%test3_ct; `%test3_cb;`%test3_ct_importable]]; trefl ()))]
+// let test3 : src_interface = {
+//   pi = test3_pi; phi = test3_phi;
+//   ct = test3_ct; ct_rcs = test3_rcs; ct_importable = test3_ct_importable; 
+//   psi = (fun _ _ _ -> True);
+// }
+// 
+// val test3_prog : prog_src test3
+// let test3_prog #fl ctx () : MIO int (IOActions + fl) (fun _ -> True) (fun _ _ _ -> True) =
+//   match static_cmd true Openfile "test.txt" with
+//   | Inl fd -> begin
+//     match ctx fd with
+//     | Inl cb -> let _ : resexn unit = cb fd in 0
+//     | Inr err -> -1
+//     end
+//   | Inr err -> -1
+// 
+// val test3_ctx : ctx_src test3 
+// let test3_ctx #fl io_acts eff_rcs fd = 
+//   Inl (fun (fd:file_descr) -> Inl () <: (MIOwp (resexn unit) fl trivial_hist))
+// 
+// val test3_ctx_t : ctx_tgt (comp_int_src_tgt test3)
+// let test3_ctx_t #fl io_acts fd : MIOpi (resexn (file_descr -> MIOpi (resexn unit) fl test3_pi)) fl test3_pi = 
+//   Inl (fun (fd:file_descr) -> Inl () <: (MIOpi (resexn unit) fl test3_pi))
