io/Compiler.Model.fst
@@ -11,13 +11,13 @@ include Compiler.Languages
 include Compiler.MIO.To.Weak
 open MIO.Behavior
 
-type policy (pi:policy_spec) =
-  h:trace -> cmd:io_cmds -> arg:io_sig.args cmd -> r:bool{r ==> pi h false cmd arg}
+type policy (mst:mst) (pi:policy_spec) =
+  s:mst.cst -> cmd:io_cmds -> arg:io_sig.args cmd -> r:bool{r ==> (forall h. mst.models s h ==> pi h false cmd arg)}
 
-type acts (fl:erased tflag) (pi:policy_spec) (caller:bool) =
+type acts (mst:mst) (fl:erased tflag) (pi:policy_spec) (caller:bool) =
   (cmd : io_cmds) ->
   (arg : io_sig.args cmd) ->
-  MIO (io_resm cmd arg) fl
+  MIO (io_resm cmd arg) mst fl
     (requires (fun _ -> True))
     (ensures (fun h r lt ->
       enforced_locally pi h lt /\
@@ -25,42 +25,46 @@ type acts (fl:erased tflag) (pi:policy_spec) (caller:bool) =
        | Inr Contract_failure -> lt == []
        | r' -> lt == [convert_call_to_event caller cmd arg r'])))
 
-type acts' (fl:erased tflag) (#pi:policy_spec) (phi:policy pi) (caller:bool) =
+type acts' (mst:mst) (fl:erased tflag) (#pi:policy_spec) (phi:policy mst pi) (caller:bool) =
   (cmd : io_cmds) ->
   (arg : io_sig.args cmd) ->
-  MIO (io_resm cmd arg) fl
+  MIO (io_resm cmd arg) mst fl
     (requires (fun _ -> True))
     (ensures (fun h r lt ->
       enforced_locally pi h lt /\
-      enforced_locally (fun h _ cmd arg -> phi h cmd arg) h lt /\
+      //enforced_locally (fun h _ cmd arg -> phi h cmd arg) h lt /\
+      // ^ really needed?
       (match r with
        | Inr Contract_failure -> lt == []
        | r' -> lt == [convert_call_to_event caller cmd arg r'])))
 
-val inst_io_cmds : #pi:policy_spec -> phi:policy pi -> acts' AllActions phi false
+val inst_io_cmds : #mst:mst -> #pi:policy_spec -> phi:policy mst pi -> acts' mst AllActions phi false
+
+#push-options "--compat_pre_core 1"
 let inst_io_cmds phi cmd arg = 
-  let h = get_trace true in
+  let h = get_state true in
   if phi h cmd arg then (
     // Need the letbinding here it won't typecheck... why?
     let r : io_resm' cmd arg = static_cmd false cmd arg in
     r
   ) else Inr Contract_failure
+#pop-options
 
 (** **** interfaces **)
 noeq
-type src_interface = {
+type src_interface (mst:mst) = {
   (* pi is in Type0 and it is used at the level of the spec,
      it describes both the events done by the partial program and the context **)
   pi : policy_spec;
   (* phi is in bool and it is used to enforce the policy on the context,
      it describes only the events of the context and it has to imply pi **)
-  phi : policy pi;
+  phi : policy mst pi;
 
   (** The type of the "context" --- not sure if it is the best name.
       It is more like the type of the interface which the two share to communicate. **)
   ct : erased tflag -> Type;
-  ct_rcs : tree pck_rc;
-  ct_importable : fl:erased tflag -> safe_importable (ct fl) pi ct_rcs fl;
+  ct_rcs : tree (pck_rc mst);
+  ct_importable : fl:erased tflag -> safe_importable (ct fl) mst pi ct_rcs fl;
 
   (** The partial program can have a post-condition that becomes the
       post-condition of the whole program after linking in the source.
@@ -69,51 +73,51 @@ type src_interface = {
 }
 
 noeq
-type tgt_interface = {
+type tgt_interface (mst:mst) = {
   pi : policy_spec;
-  phi : policy pi;
+  phi : policy mst pi;
 
   ct : erased tflag -> Type u#a;
-  ct_weak : fl:erased tflag -> weak (ct fl) fl pi;
+  ct_weak : fl:erased tflag -> weak (ct fl) mst fl pi;
 }
   
 (** **** languages **)
-type ctx_src (i:src_interface)  = #fl:erased tflag -> acts' fl i.phi false -> typ_eff_rcs fl i.ct_rcs -> i.ct fl
-type prog_src (i:src_interface) = #fl:erased tflag -> i.ct (IOActions + fl) -> unit -> MIO int (IOActions + fl) (fun _ -> True) i.psi
-type whole_src = post:(trace -> int -> trace -> Type0) & (unit -> MIO int AllActions (fun _ -> True) post)
+type ctx_src mst (i:src_interface mst)  = #fl:erased tflag -> acts' mst fl i.phi false -> typ_eff_rcs mst fl i.ct_rcs -> i.ct fl
+type prog_src mst (i:src_interface mst) = #fl:erased tflag -> i.ct (IOActions + fl) -> unit -> MIO int mst (IOActions + fl) (fun _ -> True) i.psi
+type whole_src = mst:mst & post:(trace -> int -> trace -> Type0) & (unit -> MIO int mst AllActions (fun _ -> True) post)
 
-let link_src (#i:src_interface) (p:prog_src i) (c:ctx_src i) : whole_src = 
-  (| i.psi, p #AllActions (c #AllActions (inst_io_cmds i.phi) (make_rcs_eff i.ct_rcs)) |)
+let link_src #mst (#i:src_interface mst) (p:prog_src mst i) (c:ctx_src mst i) : whole_src = 
+  (| mst, i.psi, p #AllActions (c #AllActions (inst_io_cmds i.phi) (make_rcs_eff i.ct_rcs)) |)
 
 val beh_src : whole_src ^-> trace_property #event
-let beh_src = on_domain whole_src (fun (| _, ws |) -> beh ws)
+let beh_src = on_domain whole_src (fun (| mst, _, ws |) -> beh mst ws)
 
-let src_language : language = {
-  interface = src_interface;
-  ctx = ctx_src; pprog = prog_src; whole = whole_src;
+let src_language (mst:mst) : language = {
+  interface = src_interface mst;
+  ctx = ctx_src mst; pprog = prog_src mst; whole = whole_src;
   link = link_src;
   event_typ = event;  beh = beh_src; 
 }
 
-type ctx_tgt (i:tgt_interface) = #fl:erased tflag -> acts fl i.pi false -> i.ct fl
-type prog_tgt (i:tgt_interface) = i.ct AllActions -> unit -> MIO int AllActions (fun _ -> True) (fun _ _ _ -> True)
-type whole_tgt = unit -> MIO int AllActions (fun _ -> True) (fun _ _ _ -> True)
+type ctx_tgt mst (i:tgt_interface mst) = #fl:erased tflag -> acts mst fl i.pi false -> i.ct fl
+type prog_tgt mst (i:tgt_interface mst) = i.ct AllActions -> unit -> MIO int mst AllActions (fun _ -> True) (fun _ _ _ -> True)
+type whole_tgt mst = unit -> MIO int mst AllActions (fun _ -> True) (fun _ _ _ -> True)
 
-let link_tgt (#i:tgt_interface) (p:prog_tgt i) (c:ctx_tgt i) : whole_tgt =
+let link_tgt #mst (#i:tgt_interface mst) (p:prog_tgt mst i) (c:ctx_tgt mst i) : whole_tgt mst =
   p (c #AllActions (inst_io_cmds i.phi))
 
-val beh_tgt : whole_tgt ^-> trace_property #event
-let beh_tgt = beh 
+val beh_tgt : #mst:mst -> whole_tgt mst ^-> trace_property #event
+let beh_tgt #mst = beh mst
 
-let tgt_language : language = {
-  interface = tgt_interface;
-  ctx = ctx_tgt; pprog = prog_tgt; whole = whole_tgt;
+let tgt_language (mst:mst) : language = {
+  interface = tgt_interface mst;
+  ctx = ctx_tgt mst; pprog = prog_tgt mst; whole = whole_tgt mst;
   link = link_tgt;
   event_typ = event; beh = beh_tgt; 
 }
 
 (** ** Compile interfaces **)
-let comp_int_src_tgt (i:src_interface) : tgt_interface = {
+let comp_int_src_tgt mst (i:src_interface mst) : tgt_interface mst = {
   ct = (fun fl -> (i.ct_importable fl).swtyp);
   ct_weak = (fun fl -> (i.ct_importable fl).c_swtyp);
 
@@ -122,23 +126,23 @@ let comp_int_src_tgt (i:src_interface) : tgt_interface = {
 }
 
 (** ** Compilation **)
-val backtranslate_ctx : (#i:src_interface) -> (c_t:ctx_tgt (comp_int_src_tgt i)) -> src_language.ctx i
-let backtranslate_ctx #i c_t #fl acts eff_rcs =
+val backtranslate_ctx : #mst:mst -> (#i:src_interface mst) -> (c_t:ctx_tgt mst (comp_int_src_tgt mst i)) -> (src_language mst).ctx i
+let backtranslate_ctx #mst #i c_t #fl acts eff_rcs =
   (i.ct_importable fl).safe_import (c_t #fl acts) eff_rcs
 
-val compile_whole : whole_src -> whole_tgt
-let compile_whole (| _, ws |) = ws
+val compile_whole : s:whole_src -> whole_tgt s._1
+let compile_whole (| _, _, ws |) = ws
 
-val compile_pprog : (#i:src_interface) -> (p_s:prog_src i) -> prog_tgt (comp_int_src_tgt i)
-let compile_pprog #i p_s c_t = 
+val compile_pprog : #mst:mst -> (#i:src_interface mst) -> (p_s:prog_src mst i) -> prog_tgt mst (comp_int_src_tgt mst i)
+let compile_pprog #mst #i p_s c_t = 
   let eff_rcs = make_rcs_eff i.ct_rcs in
   let c_s : i.ct AllActions = (i.ct_importable AllActions).safe_import c_t eff_rcs in
-  let ws : whole_src = (| i.psi, p_s #AllActions c_s |) in
-  let wt : whole_tgt = compile_whole ws in
+  let ws : whole_src = (| mst, i.psi, p_s #AllActions c_s |) in
+  let wt : whole_tgt mst = compile_whole ws in
   wt
 
-val compile_ctx : (#i:src_interface) -> (c_s:ctx_src i) -> ctx_tgt (comp_int_src_tgt i)
-let compile_ctx #i c_s = 
+val compile_ctx : #mst:mst -> (#i:src_interface mst) -> (c_s:ctx_src mst i) -> ctx_tgt mst (comp_int_src_tgt mst i)
+let compile_ctx #mst #i c_s = 
   (** TODO: the context should be also exportable besides importable,
       which would be a pain because one has to define a second tree of rcs. **)
 
@@ -149,11 +153,11 @@ let compile_ctx #i c_s =
       LawImportableExportable.fst **)
   admit ()
 
-let comp : compiler = {
-  source = src_language;
-  target = tgt_language;
+let comp (mst:mst) : compiler = {
+  source = src_language mst;
+  target = tgt_language mst;
 
-  comp_int = comp_int_src_tgt;
+  comp_int = comp_int_src_tgt mst;
 
   compile_pprog = compile_pprog;
 
@@ -161,49 +165,49 @@ let comp : compiler = {
 }
 
 (** ** Soundness **)
-let soundness (i:src_interface) (ct:ctx_tgt (comp_int_src_tgt i)) (ps:prog_src i) : Lemma (
-  let it = comp_int_src_tgt i in
-  let cs : ctx_src i = backtranslate_ctx #i ct in
-  let pt : prog_tgt it = (compile_pprog #i ps) in
-  let wt : whole_tgt = (pt `link_tgt` ct) in
+let soundness (mst:mst) (i:src_interface mst) (ct:ctx_tgt mst (comp_int_src_tgt mst i)) (ps:prog_src mst i) : Lemma (
+  let it = comp_int_src_tgt mst i in
+  let cs : ctx_src mst i = backtranslate_ctx #mst #i ct in
+  let pt : prog_tgt mst it = (compile_pprog #mst #i ps) in
+  let wt : whole_tgt mst = (pt `link_tgt` ct) in
   let ws : whole_src = (ps `link_src` cs) in
-  tgt_language.beh (wt) `subset_of` src_language.beh (ws) 
+  (tgt_language mst).beh (wt) `subset_of` (src_language mst).beh (ws) 
 ) = ()
 
 (** ** RrHC **)
-let syntactic_equality (i:src_interface) (ct:ctx_tgt (comp_int_src_tgt i)) (ps:prog_src i) : Lemma (
-  let it = comp_int_src_tgt i in
-  let cs : ctx_src i = backtranslate_ctx #i ct in
-  let pt : prog_tgt it = (compile_pprog #i ps) in
-  let wt : whole_tgt = (pt `link_tgt` ct) in
+let syntactic_equality (mst:mst) (i:src_interface mst) (ct:ctx_tgt mst (comp_int_src_tgt mst i)) (ps:prog_src mst i) : Lemma (
+  let it = comp_int_src_tgt mst i in
+  let cs : ctx_src mst i = backtranslate_ctx #mst #i ct in
+  let pt : prog_tgt mst it = (compile_pprog #mst #i ps) in
+  let wt : whole_tgt mst = (pt `link_tgt` ct) in
   let ws : whole_src = (ps `link_src` cs) in
   compile_whole ws == wt
 ) = ()
   
-let comp_rrhc_2 (i:src_interface) (ct:ctx_tgt (comp_int_src_tgt i)) (ps:prog_src i) : Lemma (
-  let it = comp_int_src_tgt i in
-  let cs : ctx_src i = backtranslate_ctx #i ct in
-  let pt : prog_tgt it = (compile_pprog #i ps) in
-  let wt : whole_tgt = (pt `link_tgt` ct) in
+let comp_rrhc_2 (mst:mst) (i:src_interface mst) (ct:ctx_tgt mst (comp_int_src_tgt mst i)) (ps:prog_src mst i) : Lemma (
+  let it = comp_int_src_tgt mst i in
+  let cs : ctx_src mst i = backtranslate_ctx #mst #i ct in
+  let pt : prog_tgt mst it = (compile_pprog #mst #i ps) in
+  let wt : whole_tgt mst = (pt `link_tgt` ct) in
   let ws : whole_src = (ps `link_src` cs) in
   beh_src ws == beh_tgt wt) = 
-  syntactic_equality i ct ps
+  syntactic_equality mst i ct ps
 
-let comp_rrhc_1 (i:comp.source.interface) (ct:comp.target.ctx (comp.comp_int i)) (ps:comp.source.pprog i) : Lemma (
-  let cs : comp.source.ctx i = backtranslate_ctx #i ct in
-  comp.source.beh (ps `comp.source.link #i` cs) `comp.rel_traces` comp.target.beh (comp.compile_pprog #i ps `comp.target.link #(comp.comp_int i)` ct)) =
-  comp_rrhc_2 i ct ps
+let comp_rrhc_1 (mst:mst) (i:(comp mst).source.interface) (ct:(comp mst).target.ctx ((comp mst).comp_int i)) (ps:(comp mst).source.pprog i) : Lemma (
+  let cs : (comp mst).source.ctx i = backtranslate_ctx #mst #i ct in
+  (comp mst).source.beh (ps `(comp mst).source.link #i` cs) `(comp mst).rel_traces` (comp mst).target.beh ((comp mst).compile_pprog #i ps `(comp mst).target.link #((comp mst).comp_int i)` ct)) =
+  comp_rrhc_2 mst i ct ps
   
-let comp_rrhc_0 (i:comp.source.interface) (ct:comp.target.ctx (comp.comp_int i)) : Lemma (
-      exists (cs:comp.source.ctx i).
-        forall (ps:comp.source.pprog i).
-          comp.source.beh (ps `comp.source.link #i` cs) `comp.rel_traces` comp.target.beh (comp.compile_pprog #i ps `comp.target.link #(comp.comp_int i)` ct)) = 
- introduce exists (cs:comp.source.ctx i).
-        (forall (ps:comp.source.pprog i).
-          comp.source.beh (ps `comp.source.link #i` cs) `comp.rel_traces` comp.target.beh (comp.compile_pprog #i ps `comp.target.link #(comp.comp_int i)` ct)) 
-  with (backtranslate_ctx #i ct)
-  and Classical.forall_intro (comp_rrhc_1 i ct)
+let comp_rrhc_0 (mst:mst) (i:(comp mst).source.interface) (ct:(comp mst).target.ctx ((comp mst).comp_int i)) : Lemma (
+      exists (cs:(comp mst).source.ctx i).
+        forall (ps:(comp mst).source.pprog i).
+          (comp mst).source.beh (ps `(comp mst).source.link #i` cs) `(comp mst).rel_traces` (comp mst).target.beh ((comp mst).compile_pprog #i ps `(comp mst).target.link #((comp mst).comp_int i)` ct)) = 
+ introduce exists (cs:(comp mst).source.ctx i).
+        (forall (ps:(comp mst).source.pprog i).
+          (comp mst).source.beh (ps `(comp mst).source.link #i` cs) `(comp mst).rel_traces` (comp mst).target.beh ((comp mst).compile_pprog #i ps `(comp mst).target.link #((comp mst).comp_int i)` ct)) 
+  with (backtranslate_ctx #mst #i ct)
+  and Classical.forall_intro (comp_rrhc_1 mst i ct)
           
-val comp_rrhc : unit -> Lemma (rrhc comp)
-let comp_rrhc () : Lemma (rrhc comp) by (norm [delta_only [`%rrhc]]) = 
-  Classical.forall_intro_2 (comp_rrhc_0)
+val comp_rrhc : mst:mst -> Lemma (rrhc (comp mst))
+let comp_rrhc mst : Lemma (rrhc (comp mst)) by (norm [delta_only [`%rrhc]]) = 
+  Classical.forall_intro_2 (comp_rrhc_0 mst)
